skip record typing, start subtyping (maybe)

theories/typing/examples/records.v
@@ -3,7 +3,7 @@ From iris.algebra Require Import auth.
 From lrust.lang Require Export heap.
 From lrust.lang Require Import proofmode notation.
 From lrust.typing Require Export type.
-From lrust.typing Require Import record int bool.
+From lrust.typing Require Import typing.
 From iris.prelude Require Import options.
 
 Section record.
@@ -11,7 +11,7 @@ Context `{!typeGS Σ}.
 Notation iProp := (iProp Σ).
 
 Definition re1 := rnil%E.
-Definition re2 := ("i1" /: #1 + #2 :+: "i2" /: #2 :+: rnil)%E.
+Definition re2 := ("i1" r: #1 + #2 :r: "i2" r: #2 :r: rnil)%E.
 Definition record_type := record [("x", int); ("y", int); ("z", bool)].
 
 Example re1_spec: ⊢ WP re1 {{ v, ⌜ v = RecordVNil ⌝ } }.
@@ -20,9 +20,59 @@ rewrite /re1.
 by iApply wp_value.
 Qed.
 
-Example re2_spec: ⊢ WP re2 {{ v,  ⌜ v = ("i1" /: #3 :+: "i2" /: #2 :+: rnil)%V ⌝ }}.
+Example re2_spec: ⊢ WP re2 {{ v,  ⌜ v = ("i1" r: #3 :r: "i2" r: #2 :r: rnil)%V ⌝ }}.
 Proof.
 rewrite /re2.
 by wp_op.
 Qed.
 End record.
+
+Section typing.
+Context `{!typeGS Σ}.
+
+Definition prod_pre t : type := Π [int; int; box t].
+Definition prod_cont : TypeContractive prod_pre.
+Proof.
+    intros n p1 p2 Hp.
+    rewrite /prod_pre. f_equiv.
+    f_equiv.
+    repeat f_equiv. apply Hp.
+Qed.
+
+Definition record_proper n ls : Proper (Forall2 (type_dist2 n) ==> type_dist2 n) 
+  (λ ts, record (zip ls ts)).
+Proof.
+  (*
+  If induction_arg is a natural, 
+  then destruct natural behaves like 
+  intros until natural 
+  followed by destruct applied to 
+  the last introduced hypothesis.
+  *)
+  intros ???.
+  (* KEY! *)
+  generalize dependent ls.
+  induction H. (* induction on H, not the other list types *)
+  - reflexivity.
+  - destruct ls.
+    + f_equal.
+    + assert (∀ A B (x : A) (y : B) xs ys, zip (x :: xs) (y :: ys) = (x,y) :: zip xs ys); first done. 
+      do 2 rewrite H1.
+      apply rcons_proper; first apply H. apply IHForall2.
+Qed.
+
+Definition obj_pre t : type := record [("x", int); ("y", int); ("area", box t)].
+Local Instance  obj_contractive : TypeContractive obj_pre.
+Proof.
+    intros n o1 o2 Ho.
+    rewrite /obj_pre.
+    replace ([("x", int); ("y", int); ("area", box o1)]) with (zip ["x"; "y"; "area"] [int; int; box o1]); last done.
+    replace ([("x", int); ("y", int); ("area", box o2)]) with (zip ["x"; "y"; "area"] [int; int; box o2]); last done.
+    apply record_proper.
+    repeat f_equiv.
+    apply Ho.
+Qed.
+
+Definition obj := type_fixpoint obj_pre.
+(* TODO *)
+End typing.
