theories/typing/typing.v
@@ -2,5 +2,5 @@ From lrust.lang Require Export tactics memcpy notation.
 From lrust.typing Require Export
   lft_contexts type_context cont_context programs cont type
   int bool own uniq_bor shr_bor uninit product sum fixpoint function
-  product_split borrow type_sum.
+  product_split borrow type_sum record.
 From iris.prelude Require Import options.
